src/WeierstrassCurve/WeierstrassCurveTheorems.v
@@ -3,13 +3,14 @@ Require Import Coq.Classes.Morphisms.
 Require Import Crypto.Spec.WeierstrassCurve.
 Require Import Crypto.Algebra Crypto.Algebra.Field.
 Require Import Crypto.Util.Decidable Crypto.Util.Tactics.
+Require Import BinPos.
 
 Module W.
   Section W.
     Context {F Feq Fzero Fone Fopp Fadd Fsub Fmul Finv Fdiv} {a b:F}
             {field:@Algebra.field F Feq Fzero Fone Fopp Fadd Fsub Fmul Finv Fdiv}
-            {char_gt_2:@Ring.char_gt F Feq Fzero Fone Fopp Fadd Fsub Fmul 2}
-            {char_huge:@Ring.char_gt F Feq Fzero Fone Fopp Fadd Fsub Fmul 35481600} (* TODO: we need only 3, but we may need to factor some coefficients *)
+            {char_gt_3:@Ring.char_gt F Feq Fzero Fone Fopp Fadd Fsub Fmul (BinNat.N.succ_pos (BinNat.N.two))}
+            {char_gt_11:@Ring.char_gt F Feq Fzero Fone Fopp Fadd Fsub Fmul 11%positive} (* FIXME: we shouldn't need this *)
             {Feq_dec:DecidableRel Feq}.
     Local Infix "=" := Feq : type_scope. Local Notation "a <> b" := (not (a = b)) : type_scope.
     Local Notation "0" := Fzero.  Local Notation "1" := Fone.
